examples/lowparse/LowParse.Impl.FLBytes.fst
@@ -36,3 +36,23 @@ let validate_flbytes_nochk
   (len: U32.t)
 : Tot (stateful_validator_nochk (parse_flbytes p (U32.v len)))
 = validate_constant_size_nochk len (parse_flbytes p (U32.v len))
+
+inline_for_extraction
+let validate_flbytes_consumes_all
+  (#b: bool)
+  (#t: Type0)
+  (#p: parser' b t)
+  (ps: stateful_validator p { consumes_all p } )
+  (len: U32.t)
+: Tot (stateful_validator (parse_flbytes p (U32.v len)))
+= fun (input: S.bslice) ->
+  let blen = S.length input in
+  if U32.lt blen len
+  then begin
+    None
+  end else begin
+    let input'  = S.truncate_slice input len in
+    match ps input' with
+    | Some _ -> Some (len <: consumed_slice_length input)
+    | _ -> None
+  end
